src/Lean/Compiler/LCNF/PassManager.lean
@@ -12,34 +12,34 @@ public section
 
 namespace Lean.Compiler.LCNF
 
-@[expose] def PassPhase.toNat : PassPhase → Nat
+@[expose] def Phase.toNat : Phase → Nat
   | .base => 0
   | .mono => 1
   | .impure => 2
 
-instance : ToString PassPhase where
+instance : ToString Phase where
   toString
     | .base => "base"
     | .mono => "mono"
     | .impure => "impure"
 
-def PassPhase.withPurityCheck [Inhabited α] (pp : PassPhase) (ip : Purity)
+def Phase.withPurityCheck [Inhabited α] (pp : Phase) (ip : Purity)
     (x : pp.toPurity = ip → α) : α :=
   if h : pp.toPurity = ip then
     x h
   else
     panic! s!"Compiler error: {pp} is not equivalent to IR phase {ip}, this is a bug"
 
-instance : LT PassPhase where
+instance : LT Phase where
   lt l r := l.toNat < r.toNat
 
-instance : LE PassPhase where
+instance : LE Phase where
   le l r := l.toNat ≤ r.toNat
 
-instance {p1 p2 : PassPhase} : Decidable (p1 < p2) := Nat.decLt p1.toNat p2.toNat
-instance {p1 p2 : PassPhase} : Decidable (p1 ≤ p2) := Nat.decLe p1.toNat p2.toNat
+instance {p1 p2 : Phase} : Decidable (p1 < p2) := Nat.decLt p1.toNat p2.toNat
+instance {p1 p2 : Phase} : Decidable (p1 ≤ p2) := Nat.decLe p1.toNat p2.toNat
 
-@[simp] theorem Phase.le_refl (p : PassPhase) : p ≤ p := by
+@[simp] theorem Phase.le_refl (p : Phase) : p ≤ p := by
   cases p <;> decide
 
 /--
@@ -56,11 +56,11 @@ structure Pass where
   /--
   Which phase this `Pass` is supposed to run in
   -/
-  phase : PassPhase
+  phase : Phase
   /--
   Resulting phase.
   -/
-  phaseOut : PassPhase := phase
+  phaseOut : Phase := phase
   phaseInv : phaseOut ≥ phase := by simp +arith +decide
   /--
   Whether IR validation checks should always run after this pass, regardless
@@ -85,7 +85,7 @@ of type `PassInstaller` with the `cpass` attribute.
 -/
 structure PassInstaller where
   /-- Affected phase. -/
-  phase : PassPhase
+  phase : Phase
   /--
   When the installer is run this function will receive a list of all
   current `Pass`es and return a new one, this can modify the list (and
@@ -106,7 +106,7 @@ structure PassManager where
 
 namespace Pass
 
-def mkPerDeclaration (name : Name) (phase : PassPhase)
+def mkPerDeclaration (name : Name) (phase : Phase)
     (run : Decl phase.toPurity → CompilerM (Decl phase.toPurity)) (occurrence : Nat := 0) : Pass where
   occurrence := occurrence
   phase := phase
@@ -117,7 +117,7 @@ end Pass
 
 namespace PassManager
 
-private def validatePasses (phase : PassPhase) (passes : Array Pass) : CoreM Unit := do
+private def validatePasses (phase : Phase) (passes : Array Pass) : CoreM Unit := do
   for pass in passes do
     if pass.phase != phase then
       throwError s!"{pass.name} has phase {pass.phase} but should have {phase}"
@@ -141,15 +141,15 @@ end PassManager
 
 namespace PassInstaller
 
-def installAtEnd (phase : PassPhase) (p : Pass) : PassInstaller where
+def installAtEnd (phase : Phase) (p : Pass) : PassInstaller where
   phase
   install passes := return passes.push p
 
-def append (phase : PassPhase) (passesNew : Array Pass) : PassInstaller where
+def append (phase : Phase) (passesNew : Array Pass) : PassInstaller where
   phase
   install passes := return passes ++ passesNew
 
-def withEachOccurrence (phase : PassPhase) (targetName : Name) (f : Nat → PassInstaller) : PassInstaller where
+def withEachOccurrence (phase : Phase) (targetName : Name) (f : Nat → PassInstaller) : PassInstaller where
   phase
   install passes := do
     let ⟨lowestOccurrence, highestOccurrence⟩ ← PassManager.findOccurrenceBounds targetName passes
@@ -161,7 +161,7 @@ def withEachOccurrence (phase : PassPhase) (targetName : Name) (f : Nat → Pass
       passes ← installer.install passes
     return passes
 
-def installAfter (phase : PassPhase) (targetName : Name) (p : Pass → Pass) (occurrence : Nat := 0) : PassInstaller where
+def installAfter (phase : Phase) (targetName : Name) (p : Pass → Pass) (occurrence : Nat := 0) : PassInstaller where
   phase
   install passes :=
     if let some idx := passes.findFinIdx? (fun p => p.name == targetName && p.occurrence == occurrence) then
@@ -170,10 +170,10 @@ def installAfter (phase : PassPhase) (targetName : Name) (p : Pass → Pass) (oc
     else
       throwError s!"Tried to insert pass after {targetName}, occurrence {occurrence} but {targetName} is not in the pass list"
 
-def installAfterEach (phase : PassPhase) (targetName : Name) (p : Pass → Pass) : PassInstaller :=
+def installAfterEach (phase : Phase) (targetName : Name) (p : Pass → Pass) : PassInstaller :=
     withEachOccurrence phase targetName (installAfter phase targetName p ·)
 
-def installBefore (phase : PassPhase) (targetName : Name) (p : Pass → Pass) (occurrence : Nat := 0): PassInstaller where
+def installBefore (phase : Phase) (targetName : Name) (p : Pass → Pass) (occurrence : Nat := 0): PassInstaller where
   phase
   install passes :=
     if let some idx := passes.findFinIdx? (fun p => p.name == targetName && p.occurrence == occurrence) then
@@ -182,16 +182,16 @@ def installBefore (phase : PassPhase) (targetName : Name) (p : Pass → Pass) (o
     else
       throwError s!"Tried to insert pass after {targetName}, occurrence {occurrence} but {targetName} is not in the pass list"
 
-def installBeforeEachOccurrence (phase : PassPhase) (targetName : Name) (p : Pass → Pass) : PassInstaller :=
+def installBeforeEachOccurrence (phase : Phase) (targetName : Name) (p : Pass → Pass) : PassInstaller :=
     withEachOccurrence phase targetName (installBefore phase targetName p ·)
 
-def replacePass (phase : PassPhase) (targetName : Name) (p : Pass → Pass) (occurrence : Nat := 0) : PassInstaller where
+def replacePass (phase : Phase) (targetName : Name) (p : Pass → Pass) (occurrence : Nat := 0) : PassInstaller where
   phase
   install passes := do
     let some idx := passes.findIdx? (fun p => p.name == targetName && p.occurrence == occurrence) | throwError s!"Tried to replace {targetName}, occurrence {occurrence} but {targetName} is not in the pass list"
     return passes.modify idx p
 
-def replaceEachOccurrence (phase : PassPhase) (targetName : Name) (p : Pass → Pass) : PassInstaller :=
+def replaceEachOccurrence (phase : Phase) (targetName : Name) (p : Pass → Pass) : PassInstaller :=
     withEachOccurrence phase targetName (replacePass phase targetName p ·)
 
 def run (manager : PassManager) (installer : PassInstaller) : CoreM PassManager := do
